VerificationSetCover_simple.dfy
@@ -5,7 +5,7 @@ include "Lemmas.dfy"
 method verifySetCover<T>(U:set<T>, S:set<set<T>>, k:nat, I:set<set<T>>) returns (b:bool, ghost counter:nat)   
 requires forall s | s in S :: s <= U
 ensures b == (I <= S && isCover(U, I) && |I| <= k)
-ensures counter <= |U| + 2 + |U| + |S|*|U|*|U| + |U|*|U| + 2*|U| + |I|*|U|*|S|*|U| + |I|*|U|*2*|U| + |I|*|U|*1
+ensures counter <= poly(U, S, k)
 {
   counter := 0;
   var U' := U;
@@ -27,13 +27,42 @@ ensures counter <= |U| + 2 + |U| + |S|*|U|*|U| + |U|*|U| + 2*|U| + |I|*|U|*|S|*|
     b1, U', counter := verifySetCover_outer_loop(U, S, k, I, U', counter);
   }
   counter := counter + 1;
+  /*
   assert counter <= |U| + 2 + |U| + |S|*|U|*|U| + |U|*|U| + 2*|U| + |I|*|U|*(|S|*|U| + 2*|U| + 1) by {
     assert counter <= |U| + 2 + (|U| - |U'|)*(1 + |S|*|U| + |U| + 2 + |I|*(|S|*|U| + 2*|U| + 1));
     assert counter <= |U| + 2 + (|U|)*(1 + |S|*|U| + |U| + 2 + |I|*(|S|*|U| + 2*|U| + 1));
   }
+  */
+  assert counter <= (k + 1)*|S|*|U|*|U| + (2*k + 1)*|U|*|U| + (4 + k)*|U| + 2 by {
+    assert counter <= |U| + 2 + (|U| - |U'|)*(1 + |S|*|U| + |U| + 2 + |I|*(|S|*|U| + 2*|U| + 1));
+    counter_simplification(U, S, k, I, U');
+  }
 
   assert b1 ==> U-U' == U;
   b := b1 && I <= S && |I| <= k;
+}
+
+lemma counter_simplification<T>(U:set<T>, S:set<set<T>>, k:nat, I:set<set<T>>, U':set<T>)
+requires forall s | s in S :: s <= U
+requires |I| <= k
+requires U' <= U
+ensures |U| + 2 + (|U| - |U'|)*(1 + |S|*|U| + |U| + 2 + |I|*(|S|*|U| + 2*|U| + 1)) <=
+        (k + 1)*|S|*|U|*|U| + (2*k + 1)*|U|*|U| + (4 + k)*|U| + 2
+{
+  assert (1 + k)*|S|*|U|*|U| == (k + 1)*|S|*|U|*|U|;
+  assert |I|*|U|*(|S|*|U| + 2*|U| + 1) <= k*|U|*(|S|*|U| + 2*|U| + 1) by {
+    assert |I|*|U| <= k*|U|;
+  }
+  calc <= {
+    |U| + 2 + (|U| - |U'|)*(1 + |S|*|U| + |U| + 2 + |I|*(|S|*|U| + 2*|U| + 1));
+    |U| + 2 + (|U|)*(1 + |S|*|U| + |U| + 2 + |I|*(|S|*|U| + 2*|U| + 1));
+    |U| + 2 + |U| + |S|*|U|*|U| + |U|*|U| + 2*|U| + |I|*|U|*(|S|*|U| + 2*|U| + 1);
+    4*|U| + |S|*|U|*|U| + |U|*|U| + |I|*|U|*(|S|*|U| + 2*|U| + 1) + 2;
+    4*|U| + |S|*|U|*|U| + |U|*|U| + k*|U|*(|S|*|U| + 2*|U| + 1) + 2;
+    4*|U| + |S|*|U|*|U| + |U|*|U| + (k*|U|*|S|*|U| + k*|U|*2*|U| + k*|U|*1) + 2;
+    4*|U| + |S|*|U|*|U| + |U|*|U| + k*|S|*|U|*|U| + 2*k*|U|*|U| + k*|U| + 2;
+    (k + 1)*|S|*|U|*|U| + (2*k + 1)*|U|*|U| + (4 + k)*|U| + 2;
+  }
 }
 
 
@@ -97,3 +126,6 @@ ensures counter == counter_in + |S|*|U| + 2*|U|
   counter := counter + |S|*|U|;
 }
 
+ghost function poly<T>(U: set<T>, S: set<set<T>>, k: nat) : (o:nat) {
+  (k + 1)*|S|*|U|*|U| + (2*k + 1)*|U|*|U| + (4 + k)*|U| + 2
+}
